Merkle tree: trying to fix a proof by providing more hints

secure_api/merkle_tree/MerkleTree.New.High.Correct.Rhs.fst
@@ -48,6 +48,23 @@ let rec construct_rhs_acc j fhs acc actd =
          (S.cons rhd (fst nrhsh), snd nrhsh))
   end
 
+val construct_rhs_acc_odd:
+  j:nat ->
+  fhs:hash_ss{
+    S.length fhs = log2c j /\
+    mt_hashes_lth_inv_log j fhs} ->
+  acc:hash ->
+  actd:bool ->
+  Lemma (requires (j % 2 <> 0))
+        (ensures (let rrf = construct_rhs_acc j fhs acc actd in
+                 let nacc = if actd 
+                            then hash_2 (S.last (S.head fhs)) acc
+                            else S.last (S.head fhs) in
+                 let nrrf = construct_rhs_acc (j / 2) (S.tail fhs) nacc true in
+                 S.equal (S.tail (fst rrf)) (fst nrrf) /\
+                 snd rrf == snd nrrf))
+let construct_rhs_acc_odd j fhs acc actd = ()  
+
 val construct_rhs_acc_inv_ok_0:
   fhs:hash_ss{
     S.length fhs = 1 /\
@@ -209,7 +226,7 @@ val construct_rhs_acc_consistent:
           rhs_equiv j (fst rrf) (S.slice (fst rr) lv (lv + log2c j)) actd /\
           snd rrf == snd rr)))
         (decreases j)
-#reset-options "--z3rlimit 720 --max_fuel 1"
+#reset-options "--z3rlimit 240 --max_fuel 1"
 let rec construct_rhs_acc_consistent lv i j olds hs rhs acc actd =
   log2c_bound j (32 - lv);
   mt_olds_hs_lth_inv_ok lv i j olds hs;
@@ -229,6 +246,7 @@ let rec construct_rhs_acc_consistent lv i j olds hs rhs acc actd =
       olds hs rhs acc actd
   end
   else begin
+
     let rhd = if actd then acc else hash_init in
     let nacc = if actd
                then hash_2 (S.last (S.index hs lv)) acc
@@ -246,21 +264,16 @@ let rec construct_rhs_acc_consistent lv i j olds hs rhs acc actd =
                  (S.slice (merge_hs olds hs) (lv + 1) (lv + 1 + (log2c (j / 2))))
                  nacc true in
 
-    assert (S.equal (fst rrf) (S.cons rhd (fst nrrf)));
-    seq_tail_cons rhd (fst nrrf);
-    seq_head_cons rhd (fst nrrf);
-    assert (S.equal (S.tail (fst rrf)) (fst nrrf));
-    assert (snd rrf == snd nrrf);
+    construct_rhs_acc_odd j (S.slice (merge_hs olds hs) lv (lv + log2c j)) acc actd;
 
     // Recursion step for `construct_rhs`
     assert (hs_wf_elts (lv + 1) hs (i / 2) (j / 2));
     let nrhs = if actd then S.upd rhs lv acc else rhs in
     let nrr = construct_rhs (lv + 1) hs nrhs (i / 2) (j / 2) nacc true in
+    construct_rhs_odd lv hs rhs i j acc actd;
     construct_rhs_unchanged (lv + 1) hs nrhs (i / 2) (j / 2) nacc true;
     assert (S.equal (S.slice nrhs 0 (lv + 1)) (S.slice (fst nrr) 0 (lv + 1)));
     assert (S.index (fst nrr) lv == S.index nrhs lv);
-    assert (S.equal (fst rr) (fst nrr));
-    assert (snd rr == snd nrr);
 
     // Recursion for the proof
     construct_rhs_acc_consistent (lv + 1) (i / 2) (j / 2)
